ainvs+access+infoflow+dpolicy: interpret xn as Read on AARCH64
Introduce ptable_exec to use in do_user_op_if. It makes the execute
right available. All architectures have some form of it, but how it is
handled and whether it may imply Read authority or not differs.

Use the new interface in AARCH64 where XN implies Read authority even
for pages without read permission on the PTE. This forces the infoflow
proof to show that the XN fix from the previous commit is sufficient.

Signed-off-by: Gerwin Klein <gerwin.klein@proofcraft.systems>

proof/access-control/AARCH64/ArchAccess.thy
@@ -12,23 +12,23 @@ context Arch begin arch_global_naming
 
 subsection \<open>Arch-specific transformation of caps into authorities\<close>
 
-definition vspace_cap_rights_to_auth :: "cap_rights \<Rightarrow> auth set" where
-  "vspace_cap_rights_to_auth r \<equiv>
+definition vspace_cap_rights_to_auth :: "cap_rights \<Rightarrow> bool \<Rightarrow> auth set" where
+  "vspace_cap_rights_to_auth r exec \<equiv>
      (if AllowWrite \<in> r then {Write} else {})
-   \<union> (if AllowRead \<in> r then {Read} else {})"
+   \<union> (if AllowRead \<in> r \<or> exec then {Read} else {})"
 
 definition arch_cap_auth_conferred where
   "arch_cap_auth_conferred arch_cap \<equiv>
-     (if is_FrameCap arch_cap then vspace_cap_rights_to_auth (acap_rights arch_cap) else {Control})"
+     (if is_FrameCap arch_cap then vspace_cap_rights_to_auth (acap_rights arch_cap) False else {Control})"
 
 subsection \<open>Generating a policy from the current ASID distribution\<close>
 
 definition pte_ref2 where
   "pte_ref2 level pte \<equiv> case pte of
-     PagePTE paddr _ _ rights
+     PagePTE paddr _ attrs rights
        \<Rightarrow> Some (ptrFromPAddr paddr,
                 pt_bits_left level,
-                vspace_cap_rights_to_auth rights)
+                vspace_cap_rights_to_auth rights (Execute \<in> attrs))
    | PageTablePTE ppn
        \<Rightarrow> Some (ptrFromPAddr (paddr_from_ppn ppn), 0, {Control})
    | _ \<Rightarrow> None"
